Implemented a decision procedure for checking if an element beongs to a binomial heap. Moved the tactic inj to RCCBase.v. Fixed the definition of binomial heap. Tried to implement McCarthy's f91 function using Bove-Capretta method and partially succeeded.

Basic/BinomialTree.v
@@ -3,206 +3,6 @@ Add Rec LoadPath "/home/zeimer/Code/Coq".
 Require Export LinDec.
 Require Export RCCBase.
 
-(*Inductive BinomialTree (A : Type) : nat -> Type :=
-    | leaf : A -> BinomialTree A 0
-    | link :
-        forall (rank : nat) (l r : BinomialTree A rank),
-          BinomialTree A (S rank).*)
-
-Module wut.
-
-Inductive BinomialTree (A : Type) : nat -> Type :=
-    | leaf : A -> BinomialTree A 0
-    | forest : A -> forall {rank : nat}, BinomialForest A rank ->
-        BinomialTree A (S rank)
-
-with BinomialForest (A : Type) : nat -> Type :=
-    | bfnil : BinomialForest A 0
-    | bfcons : forall {r : nat},
-        BinomialTree A (S r) -> BinomialForest A r ->
-          BinomialForest A (S r).
-
-Arguments leaf {A} _.
-Arguments forest {A} _ {rank} _.
-Arguments bfnil {A}.
-Arguments bfcons {A r} _ _.
-
-Inductive elem {A : Type} (x : A)
-  : forall {r : nat}, BinomialTree A r -> Prop :=
-    | elem_leaf : elem x (leaf x)
-    | elem_forest_here :
-        forall (r : nat) (f : BinomialForest A r),
-          elem x (forest x f)
-    | elem_forest_there :
-        forall (y : A) (r : nat) (f : BinomialForest A r),
-          elemForest x f -> elem x (forest y f)
-
-with elemForest {A : Type} (x : A)
-  : forall {r : nat}, BinomialForest A r -> Prop :=
-    | elemForest_bfcons_tree :
-        forall (r : nat) (t : BinomialTree A (S r)) (f : BinomialForest A r),
-          elem x t -> elemForest x (bfcons t f)
-    | elemForest_bfcons_forest :
-        forall (r : nat) (t : BinomialTree A (S r)) (f : BinomialForest A r),
-          elemForest x f -> elemForest x (bfcons t f).
-
-Hint Constructors elem elemForest.
-
-Fixpoint elem_dec
-  {A : LinDec} (x : A) {r : nat} (t : BinomialTree A r) :
-    {elem x t} + {~ elem x t}
-
-with elemForest_dec
-  {A : LinDec} (x : A) {r : nat} (f : BinomialForest A r) :
-    {elemForest x f} + {~ elemForest x f}.
-Proof.
-  destruct t as [y | y r f].
-    clear - x y. case_eq (x =? y); intros; dec.
-      right. inv 1.
-    case_eq (x =? y); intros.
-      clear - x y H. dec.
-      destruct (elemForest_dec A x r f).
-        left. constructor. assumption.
-        right. inv 1.
-          dec.
-          apply inj_pair2 in H4. subst. contradiction.
-  destruct f.
-    right. inv 1.
-    destruct (elem_dec A x (S r) b).
-      left. constructor. assumption.
-      destruct (elemForest_dec A x r f).
-        left. auto.
-        right. inv 1; apply inj_pair2 in H1; apply inj_pair2 in H3; subst.
-          contradiction.
-          contradiction.
-Defined.
-
-End wut.
-
-Module wut2.
-
-Inductive BinomialTree (A : Type) : nat -> Type :=
-    | node : A -> forall {r : nat}, BinomialForest A (pred r) ->
-        BinomialTree A r
-
-with BinomialForest (A : Type) : nat -> Type :=
-    | bfnil : BinomialForest A 0
-    | bfcons : forall {r : nat},
-        BinomialTree A (S r) -> BinomialForest A r ->
-          BinomialForest A (S r).
-
-Arguments node {A} _ {r} _.
-Arguments bfnil {A}.
-Arguments bfcons {A r} _ _.
-
-Inductive elem {A : Type} (x : A)
-  : forall {r : nat}, BinomialTree A r -> Prop :=
-    | elem_here :
-        forall (r : nat) (f : BinomialForest A (pred r)),
-          elem x (node x f)
-    | elem_there :
-        forall (y : A) (r : nat) (f : BinomialForest A (pred r)),
-          elemForest x f -> elem x (node y f)
-
-with elemForest {A : Type} (x : A)
-  : forall {r : nat}, BinomialForest A r -> Prop :=
-    | elemForest_bfcons_tree :
-        forall (r : nat) (t : BinomialTree A (S r)) (f : BinomialForest A r),
-          elem x t -> elemForest x (bfcons t f)
-    | elemForest_bfcons_forest :
-        forall (r : nat) (t : BinomialTree A (S r)) (f : BinomialForest A r),
-          elemForest x f -> elemForest x (bfcons t f).
-
-Hint Constructors elem elemForest.
-
-Fixpoint elem_dec
-  {A : LinDec} (x : A) {r : nat} (t : BinomialTree A r) :
-    {elem x t} + {~ elem x t}
-
-with elemForest_dec
-  {A : LinDec} (x : A) {r : nat} (f : BinomialForest A r) :
-    {elemForest x f} + {~ elemForest x f}.
-Proof.
-  destruct t as [y r f].
-    case_eq (x =? y); intros.
-      left. dec.
-      destruct (elemForest_dec A x _ f).
-        left. auto.
-        right. inv 1.
-          dec.
-          apply inj_pair2 in H4. subst. contradiction.
-  destruct f as [| r t f'].
-    right. inv 1.
-    destruct (elem_dec A x (S r) t).
-      left. auto.
-      destruct (elemForest_dec A x _ f').
-        left. auto.
-        right. inv 1; apply inj_pair2 in H1; apply inj_pair2 in H3;
-          subst; contradiction.
-Defined.
-
-End wut2.
-
-Module wut3.
-
-Inductive BinomialTree (A : Type) : nat -> Type :=
-    | node : A -> forall {r : nat}, BinomialForest A (pred r) ->
-        BinomialTree A r
-
-with BinomialForest (A : Type) : nat -> Type :=
-    | bfnil : BinomialForest A 0
-    | bfcons : forall {r : nat},
-        BinomialTree A (S r) -> BinomialForest A r ->
-          BinomialForest A (S r).
-
-Arguments node {A} _ {r} _.
-Arguments bfnil {A}.
-Arguments bfcons {A r} _ _.
-
-Inductive elem {A : Type} (x : A)
-  : forall {r : nat}, BinomialTree A r -> Prop :=
-    | elemC :
-        forall (y : A) (r : nat) (f : BinomialForest A (pred r)),
-          x = y \/ elemForest x f -> elem x (node y f)
-
-with elemForest {A : Type} (x : A)
-  : forall {r : nat}, BinomialForest A r -> Prop :=
-    | elemForestC :
-        forall (r : nat) (t : BinomialTree A (S r)) (f : BinomialForest A r),
-          elem x t \/ elemForest x f -> elemForest x (bfcons t f).
-
-Hint Constructors elem elemForest.
-
-Fixpoint elem_dec
-  {A : LinDec} (x : A) {r : nat} (t : BinomialTree A r) :
-    {elem x t} + {~ elem x t}
-
-with elemForest_dec
-  {A : LinDec} (x : A) {r : nat} (f : BinomialForest A r) :
-    {elemForest x f} + {~ elemForest x f}.
-Proof.
-  destruct t as [y r f].
-    case_eq (x =? y); intros.
-      left. dec.
-      destruct (elemForest_dec A x _ f).
-        left. auto.
-        right. inv 1.
-          dec.
-          apply inj_pair2 in H4. inv H3.
-  destruct f as [| r t f'].
-    right. inv 1.
-    destruct (elem_dec A x _ t).
-      left. constructor. auto.
-      destruct (elemForest_dec A x _ f').
-        left. auto.
-        right. inv 1; apply inj_pair2 in H1; apply inj_pair2 in H3;
-          subst; inv H2.
-Defined.
-
-End wut3.
-
-Module wut4.
-
 Inductive BinomialTree (A : Type) : nat -> Type :=
     | node : A -> forall {r : nat}, BinomialForest A r -> BinomialTree A r
 
@@ -256,8 +56,39 @@ Proof.
           subst; inv H2.
 Defined.
 
+Fixpoint elem_decb
+  {A : LinDec} (x : A) {r : nat} (t : BinomialTree A r) : bool :=
+match t with
+    | node x' ts =>
+        (x =? x') || elemForest_decb x ts
+end
+with elemForest_decb
+  {A : LinDec} (x : A) {r : nat} (ts : BinomialForest A r) : bool :=
+match ts with
+    | bfnil => false
+    | bfcons h ts' => elem_decb x h || elemForest_decb x ts'
+end.
+
+Lemma elem_decb_spec :
+  forall (A : LinDec) (x : A) (r : nat) (t : BinomialTree A r),
+    reflect (elem x t) (elem_decb x t)
+
+with elemForest_decb_spec :
+  forall (A : LinDec) (x : A) (r : nat) (ts : BinomialForest A r),
+    reflect (elemForest x ts) (elemForest_decb x ts).
+Proof.
+  destruct t as [x' r ts]. simpl. dec.
+    destruct (elemForest_decb_spec A x r ts). auto.
+      constructor. inv 1. inj. firstorder.
+  destruct ts as [| r t ts']; simpl.
+    constructor. inv 1.
+    destruct (elem_decb_spec A x r t); auto.
+      destruct (elemForest_decb_spec A x r ts'); auto.
+        constructor. inv 1. inj. firstorder.
+Qed.
+
 Definition BinomialHeap (A : Type) : Type :=
-  {r : nat & list (BinomialTree A r)}.
+  list {r : nat & BinomialTree A r}.
 
 Print BinomialTree.
 
@@ -287,4 +118,10 @@ with
         end ts
 end t2).*)
 
-End wut4.
+Lemma link_comm :
+  forall (A : LinDec) (r : nat) (t1 t2 : BinomialTree A r),
+    link t1 t2 = link t2 t1.
+Proof.
+  destruct t1, t2. dec; assert (c = c0) by dec; subst.
+    repeat f_equal.
+Abort.
